Finish opening the inode
This was difficult because the wp_UsedBlock spec actually took a bunch
of durable state, which needed to be framed out. We should probably be
more principled about separating the two, especially for this weird code
that reads state before setting up crash conditions.

src/program_proof/examples/inode_proof.v
@@ -117,6 +117,13 @@ Proof.
   iExists _; iFrame.
 Qed.
 
+Theorem pre_inode_to_cinv l γ addr σ :
+  pre_inode l γ addr σ -∗ inode_cinv addr σ.
+Proof.
+  iNamed 1.
+  iApply inode_linv_to_cinv; iFrame.
+Qed.
+
 Global Instance is_inode_Persistent l k γ P addr :
   Persistent (is_inode l k γ P addr).
 Proof. apply _. Qed.
@@ -258,24 +265,50 @@ Proof.
   iDestruct (big_sepL2_length with "Hdata") as "$".
 Qed.
 
-Theorem wp_Inode__UsedBlocks {l γ addr σ} :
-  {{{ pre_inode l γ addr σ }}}
+Definition used_blocks_pre l σ addrs: iProp Σ :=
+  ∃ addr_s,
+    "%Haddr_set" ∷ ⌜list_to_set addrs = σ.(inode.addrs)⌝ ∗
+    "addrs" ∷ l ↦[Inode.S :: "addrs"] (slice_val addr_s) ∗
+    "Haddrs" ∷ is_slice addr_s uint64T 1 addrs.
+
+(* this lets the caller frame out the durable state for the crash invariant and
+the memory state for UsedBlocks *)
+Theorem pre_inode_read_addrs l γ addr σ :
+  pre_inode l γ addr σ -∗
+  ∃ addrs, used_blocks_pre l σ addrs ∗
+           is_inode_durable addr σ addrs ∗
+           (used_blocks_pre l σ addrs -∗
+            is_inode_durable addr σ addrs -∗
+            pre_inode l γ addr σ).
+Proof.
+  iNamed 1.
+  iNamed "Hlockinv".
+  iDestruct (is_inode_durable_addrs with "Hdurable") as "%Haddr_set".
+  iExists addrs.
+  iSplitL "addrs Haddrs".
+  { iExists _; iFrame "% ∗". }
+  iFrame.
+  iNamed 1.
+  iIntros "Hdurable".
+  iExists _, _; iFrame.
+  iExists _, _; iFrame "∗ %".
+Qed.
+
+Theorem wp_Inode__UsedBlocks {l σ addrs} :
+  {{{ used_blocks_pre l σ addrs }}}
     Inode__UsedBlocks #l
-  {{{ (s:Slice.t) (addrs: list u64), RET (slice_val s);
+  {{{ (s:Slice.t), RET (slice_val s);
       is_slice s uint64T 1 addrs ∗
       ⌜list_to_set addrs = σ.(inode.addrs)⌝ ∗
-      (is_slice s uint64T 1 addrs -∗ pre_inode l γ addr σ) }}}.
+      (is_slice s uint64T 1 addrs -∗ used_blocks_pre l σ addrs) }}}.
 Proof.
   iIntros (Φ) "Hinode HΦ"; iNamed "Hinode".
   wp_call.
-  iNamed "Hlockinv".
   wp_loadField.
   iApply "HΦ".
-  iDestruct (is_inode_durable_addrs with "Hdurable") as %Haddrs.
-  iFrame (Haddrs) "Haddrs".
-  iIntros "Hs".
-  iExists _, _; iFrame "# ∗".
-  iExists _, _; iFrame; auto.
+  iFrame "∗ %".
+  iIntros "Haddrs".
+  iExists _; iFrame.
 Qed.
 
 Theorem wpc_Inode__Read {k E2} {l γ k' P addr} {off: u64} Q :
